LgtmLean/LgtmLean.lean
@@ -5,6 +5,7 @@ module
 import LgtmLean.Basic
 import LgtmLean.CreateThreads
 import LgtmLean.Files
+import LgtmLean.Interface
 import LgtmLean.Repository
 import LgtmLean.Threads
 import LgtmLean.Tree
